Here's a breakdown of the past questions, addressing each part:

**Question 1**

*   **a.** Convert the binary number 1000100111000011 to hexadecimal and octal.
    *   **Hexadecimal:** Divide the binary number into groups of 4 bits from right to left: `1000 1001 1100 0011`. Convert each group to its hexadecimal equivalent: `8 9 C 3`. The hexadecimal representation is `89C3`.
    *   **Octal:** Divide the binary number into groups of 3 bits from right to left: `10 001 001 110 000 11`. Convert each group to its octal equivalent: `2 1 1 6 0 3`. The octal representation is `211603`.
*   **b.** Using parity coding, convert 67 (base 10) to odd parity.
    *   First, convert 67 to binary: `01000011`. Since we are using a word length of 1 byte, we'll represent it with 8 bits.
    *   **Odd Parity:** Count the number of 1s in the binary representation (`01000011`). There are two 1s. For odd parity, we need an odd number of 1s. Therefore, we will add a parity bit of '1' to the beginning. The result becomes: `101000011`.
*   **c.** Given matrix A = \[1 2 3; 5 1 4; 3 2 1], X = A(1,:), Y = A(3,:). Find X.\*Y.
    *   `X = A(1,:)` means X is the first row of A: `[1 2 3]`.
    *   `Y = A(3,:)` means Y is the third row of A: `[3 2 1]`.
    *   `X.*Y` represents element-wise multiplication (Hadamard product): `[1\*3, 2\*2, 3\*1] = [3 4 3]`.
*   **d.** Use the graphical method to solve the system of equations.
    *   x1 - 3x2 = 5
    *   2x1 - 6x2 = 7
    *   Isolate x2 for each equation
        *   x2 = (x1 - 5) / 3
        *   x2 = (2x1 - 7) / 6
    *   To sketch the lines, find some points for each equation
        *   for x2 = (x1 - 5) / 3
            *   when x1= 2, x2 = -1
            *   when x1 = 5, x2 = 0
        *   for x2 = (2x1 - 7) / 6
            *   when x1= 2, x2 = -1/6
            *   when x1 = 5, x2 = 1/2
    *   Plot the lines.  If they intersect, that's your approximate solution. Because of the nature of the equations, they are parallel lines so the graphical method will not provide an answer. In this case, you can state no solution.
*   **e.** Solve the system of equations using Gauss Elimination with pivoting.
    *   6x1 - 2x2 + 2x3 + 4x4 = 16
    *   12x1 - 8x2 + 6x3 + 10x4 = 26
    *   3x1 - 13x2 + 9x3 + 3x4 = -19
    *   -6x1 + 4x2 + x3 - 18x4 = -34

    *   **Pivoting:**  This involves rearranging the equations to have the largest coefficient (in absolute value) for the variable you're eliminating at each step.
    *   **Step 1:**  Identify the largest coefficient for x1 (it's 12 in the second equation). Swap equation 1 and 2 to have this equation in the first position.
        *   12x1 - 8x2 + 6x3 + 10x4 = 26
        *   6x1 - 2x2 + 2x3 + 4x4 = 16
        *   3x1 - 13x2 + 9x3 + 3x4 = -19
        *   -6x1 + 4x2 + x3 - 18x4 = -34
    *   **Step 2:** Eliminate x1 from equations 2, 3, and 4
        *   Divide equation 1 by 12:  x1 - (2/3)x2 + (1/2)x3 + (5/6)x4 = 13/6
        *   Equation 2:  Equation 2 - 6 \* Equation 1 :  -6x2 - x3 - x4 = -10
        *   Equation 3: Equation 3 - 3 \* Equation 1 : -11x2 + (15/2)x3 - (3/2)x4 = -77/2
        *   Equation 4: Equation 4 - (-6) \* Equation 1:  0x2 + 2x3 - 13x4 = -21
    *   **Step 3:** Divide second equation by -6: x2 + (1/6)x3 + (1/6)x4 = 5/3
    *   **Step 4:** Eliminate x2 from equation 3: equation 3 - (-11) \* equation 2 : (28/3)x3 + (4/3)x4 = -101/6
    *   **Step 5:** Eliminate x2 from equation 4: equation 4 - 0 \* equation 2: 2x3 - 13x4 = -21
    *   **Step 6:** Divide equation 3 by 28/3:  x3 + (1/7)x4 = -101/56
    *   **Step 7:** Eliminate x3 from equation 4: equation 4 - 2 \* equation 3: -93/7x4 = -277/28
    *   **Step 8:** Solve for x4: x4 = 277/372
    *   **Step 9:** Solve for x3: x3 = -101/56 - (1/7)(277/372) = -6409/2604
    *   **Step 10:** Solve for x2: x2 = 5/3 - (1/6)(-6409/2604) - (1/6)(277/372) = 17563/15624
    *   **Step 11:** Solve for x1: x1 = 13/6 + (2/3)(17563/15624) - (1/2)(-6409/2604) - (5/6)(277/372) = 171887/93744

**Question 2**

*   **a.** Pseudocode for forward elimination and backward substitution in Naive Gauss Elimination.
    *   **Forward Elimination:** This part reduces the system to an upper triangular form.  We'll use a nested loop structure.

        ```
        function forwardElimination(A, b)
            n = size(A, 1) // Number of rows (equations)
            for k = 1 to n-1 // Iterate through columns (variables to eliminate)
                for i = k+1 to n // Iterate through rows below the current one
                    factor = A[i, k] / A[k, k] // Calculate the factor
                    for j = k to n // Iterate through the columns to update
                        A[i, j] = A[i, j] - factor * A[k, j] // Eliminate the variable
                    b[i] = b[i] - factor * b[k] // Update the b vector
                end for
            end for
            return A, b // Return the modified matrix and vector
        end function
        ```

    *   **Backward Substitution:** This part solves for the variables, starting from the last one.

        ```
        function backwardSubstitution(A, b)
            n = size(A, 1)
            x = zeros(n, 1) // Initialize the solution vector
            x[n] = b[n] / A[n, n] // Solve for the last variable
            for i = n-1 down to 1 // Iterate backwards through the equations
                sum = 0
                for j = i+1 to n
                    sum = sum + A[i, j] * x[j] // Calculate the sum of known terms
                end for
                x[i] = (b[i] - sum) / A[i, i] // Solve for the current variable
            end for
            return x // Return the solution vector
        end function
        ```

*   **b.** Solve the system using Naive Gauss Elimination.

    *   6x1 - 2x2 + 2x3 + 4x4 = 16
    *   12x1 - 8x2 + 6x3 + 10x4 = 26
    *   3x1 - 13x2 + 9x3 + 3x4 = -19
    *   -6x1 + 4x2 + x3 - 18x4 = -34
    *   Follow the forward elimination and then backward substitution procedures, but without pivoting.

    *   **Step 1: Eliminate x1 from equations 2, 3, and 4:**
        *   Equation 2: Equation 2 - 2 \* Equation 1: -4x2 + 2x3 + 2x4 = -6
        *   Equation 3: Equation 3 - (1/2) \* Equation 1: -12x2 + 8x3 + x4 = -27
        *   Equation 4: Equation 4 + Equation 1: 2x2 + 3x3 - 14x4 = -18
    *   **Step 2: Eliminate x2 from equations 3 and 4**
        *   Equation 3: Equation 3 - 3 \* Equation 2: 2x3 - 5x4 = -9
        *   Equation 4: Equation 4 + (1/2) \* Equation 2: 4x3 - 13x4 = -21
    *   **Step 3: Eliminate x3 from equation 4**
        *   Equation 4: Equation 4 - Equation 3: -3x4 = -3
        *   Therefore, x4 = 1.
    *   **Step 4: Solve for x3:**
        *   2x3 - 5(1) = -9  => 2x3 = -4 => x3 = -2
    *   **Step 5: Solve for x2**
        *   -4x2 + 2(-2) + 2(1) = -6 => -4x2 = -6 + 4 - 2 => -4x2 = -4 => x2 = 1
    *   **Step 6: Solve for x1**
        *   6x1 - 2(1) + 2(-2) + 4(1) = 16 => 6x1 = 16 + 2 + 4 - 4 => 6x1 = 18 => x1 = 3

**Question 3**

*   **a.** Meanings of MATLAB commands:
    *   `who`: Lists the variables currently in the workspace.
    *   `whos`: Lists the variables in the workspace, along with their sizes, data types, and other information.
    *   `what`: Lists MATLAB-specific files (e.g., .m files, .mat files) in the current directory.
    *   `pwd`: Displays the current working directory.
*   **b.** Solve the system of equations using the Gauss-Jordan method.
    *   x - 2y + 3z = 9
    *   -x + 3y = -4
    *   2x - 5y + 5z = 17
    *   **Step 1: Augmented Matrix**
        *   Form the augmented matrix:  \[1 -2 3 | 9; -1 3 0 | -4; 2 -5 5 | 17]
    *   **Step 2: Forward Elimination (Gauss Elimination steps)**
        *   Eliminate x from the second and third rows.
            *   Add row 1 to row 2: \[1 -2 3 | 9; 0 1 3 | 5; 2 -5 5 | 17]
            *   Subtract 2 * row 1 from row 3: \[1 -2 3 | 9; 0 1 3 | 5; 0 -1 -1 | -1]
        *   Eliminate y from the third row:
            *   Add row 2 to row 3: \[1 -2 3 | 9; 0 1 3 | 5; 0 0 2 | 4]
        *   Divide row 3 by 2: \[1 -2 3 | 9; 0 1 3 | 5; 0 0 1 | 2]
    *   **Step 3: Back Substitution (Gauss-Jordan to reduced row echelon form)**
        *   Eliminate z from rows 1 and 2
            *   Subtract 3 * row 3 from row 2: \[1 -2 3 | 9; 0 1 0 | -1; 0 0 1 | 2]
            *   Subtract 3 * row 3 from row 1: \[1 -2 0 | 3; 0 1 0 | -1; 0 0 1 | 2]
        *   Eliminate y from row 1
            *   Add 2 * row 2 to row 1: \[1 0 0 | 1; 0 1 0 | -1; 0 0 1 | 2]
    *   **Step 4: Solution**
        *   From the final matrix:
            *   x = 1
            *   y = -1
            *   z = 2

**Question 4**

*   **4a.** Differentiate between Riemann Sums and Trapezoidal Sum for solving integral equations.
    *   **Riemann Sums:**  Approximates the definite integral by dividing the area under the curve into rectangles.
        *   **Left Riemann Sum:** Rectangles have heights determined by the function value at the *left* endpoint of each subinterval.
        *   **Right Riemann Sum:** Rectangles have heights determined by the function value at the *right* endpoint of each subinterval.
        *   **Midpoint Riemann Sum:** Rectangles have heights determined by the function value at the *midpoint* of each subinterval.
        *   *General Formula:*  `∫[a, b] f(x) dx ≈ Σ f(xi) * Δx`  (sum of function values at sample points times the width of each subinterval)
    *   **Trapezoidal Rule:** Approximates the definite integral by dividing the area under the curve into trapezoids.
        *   *Formula:* `∫[a, b] f(x) dx ≈ (Δx / 2) \* [f(x0) + 2f(x1) + 2f(x2) + ... + 2f(xn-1) + f(xn)]` where Δx = (b-a)/n.
        *   The trapezoidal rule is usually more accurate than the Riemann Sums (especially with the same number of intervals) because it better approximates the curve's shape by using trapezoids instead of just rectangles.
        *   For the trapezoidal sum, the area is the sum of the area of the trapezoids.

*   **4b.** Solve the differential equation  dy/dx = -y + 2cos(x), y(0) = 1  using Simpson's rule.
    *   Simpson's rule is designed for numerically approximating definite *integrals*, not directly solving differential equations.  To solve a differential equation numerically, you will likely use a method such as Euler's method, Runge-Kutta, or a similar algorithm.  There are numerical techniques that apply Simpson's rule to definite integrals, but not for differential equations.  We are going to make a few assumptions to use Simpson's rule. First we need to get the y value, and we are going to assume that this applies to one time step.
    *   **Step 1. Determine Step Size and Interval** We are going to assume a step size of h = 0.1, and interval is 0 to 0.1.
    *   **Step 2: Prepare the Values.**
        *   Initial condition: x0 = 0, y(0) = 1
        *   We need to know y at x0. Then we can use the formula to find y(x1)
        *   y'(x) = f(x, y) = -y + 2cos(x)
        *   We will want to calculate y'(0)
            *   y'(0) = -1 + 2cos(0) = -1 + 2(1) = 1
    *   **Step 3. Apply Simpson's 1/3 Rule.**  Simpson's 1/3 rule (for a single step, since we have only 2 points)

        *  y(x1) ≈ y(x0) + (h/3) \* \[y'(x0) + 4y'(x1/2) + y'(x1)]
        *  To use this form, we need to apply the derivative equation.
        *  we know x0, y(x0), h, so we need to find y'(x0), y'(x1), y'(x1/2)
        *  Find x1/2
            *   x1/2 = 0 + (0.1/2) = 0.05
        *   y'(0.05) = -y(0.05) + 2cos(0.05)
            *   We approximate y(0.05) ≈ y(0) + (0.05) * y'(0) = 1 + (0.05) \* 1 = 1.05
            *   y'(0.05) ≈ -1.05 + 2cos(0.05) = 0.95995
        *   Find x1
            *   x1 = 0 + 0.1 = 0.1
        *   y'(x1) ≈ -y(x1) + 2cos(x1)
            *   We approximate y(0.1) ≈ y(0) + (0.1) \* y'(0) = 1 + (0.1) \* 1 = 1.1
            *   y'(0.1) ≈ -1.1 + 2cos(0.1) = 0.90996
        *  y(x1) ≈ 1 + (0.1/3) \* \[1 + 4(0.95995) + 0.90996]
        *  y(0.1) ≈ 1 + 0.1 \* (1 + 3.8398 + 0.90996)/3
        *  y(0.1) ≈ 1 + 0.191658
        *  y(0.1) ≈ 1.191658

**Question 5**

*   **5a.** Given matrix A = \[2 5 3; 5 0 4; 3 2 6], X = A(:,1), Y = A(:,3). Find X.\*Y.
    *   `X = A(:,1)` means X is the first column of A: `[2; 5; 3]`.
    *   `Y = A(:,3)` means Y is the third column of A: `[3; 4; 6]`.
    *   `X.\*Y` represents element-wise multiplication: `[2\*3; 5\*4; 3\*6] = [6; 20; 18]`.
*   **5b.** Solve the problem  y'(x) = -y(x) + 2cos(x), y(0) = 1 using Euler's method.
    *   **Euler's Method:** A simple numerical method for approximating the solution of a differential equation. The formula is:  `y(x + h) ≈ y(x) + h * f(x, y)`.
        *   h = step size
    *   **Step 1: Determine the step size, h:** Let's say we want to estimate y(x) at x = 0.1 with step size of 0.1.
    *   **Step 2: Apply the formula, one step at a time:**
        *   We have:  y'(x) = -y(x) + 2cos(x)
        *   We know x0 = 0 and y(0) = 1.
        *   Using the Euler's method formula, with h = 0.1:
        *   y(0.1) ≈ y(0) + 0.1 \* f(0, y(0))
        *   f(x, y) = -y + 2cos(x)  =>  f(0, 1) = -1 + 2\*cos(0) = -1 + 2 = 1.
        *   y(0.1) ≈ 1 + 0.1 \* (1) = 1.1
        *   Therefore, after one step, the estimated value of y at x=0.1 is approximately 1.1.

